Deploying to gh-pages from @ xubaiw/reservoir-index@5d8f052174f7cf89d2d294fb431c63d74848f6d7 🚀

git/zaxioms/LeanAlg/c/ffi.c
@@ -1,0 +1,119 @@
+#include <lean/lean.h>
+#include <string.h>
+#include <stdlib.h>
+#include <stdio.h>
+
+typedef struct cVec {
+    double*   data;
+    uint32_t length;
+} cVec;
+
+//good
+static lean_external_class* g_cVec_external_class = NULL;
+
+extern lean_object* l_instInhabitedFloat;
+
+lean_obj_res make_error(const char* err_msg) {
+    return lean_mk_io_user_error(lean_mk_io_user_error(lean_mk_string(err_msg)));
+}
+//good
+void cVec_finalizer(void* v_) {
+    cVec* v = (cVec*) v_;
+    if (v->data) {
+        free(v->data);
+    }
+    free(v);
+}
+//good
+void noop_foreach(void* mod, b_lean_obj_arg fn) {}
+//good
+lean_obj_res cVec_initialize() {
+    g_cVec_external_class = lean_register_external_class(
+        cVec_finalizer,
+        noop_foreach
+    );
+    return lean_io_result_mk_ok(lean_box(0));
+}
+//good
+cVec* cVec_alloc(uint32_t length){
+    cVec* out = (cVec*) malloc(sizeof(cVec));
+    if (out == NULL) {
+        printf("Insufficient Memory\n");
+    }
+
+    out->data = (double*)(malloc(sizeof(double)*length));
+    if (out->data == NULL) {
+        printf("Insufficient Memory\n");
+    }
+    out->length = length;
+
+    return out;
+}
+
+// causing a segfault
+// Not sure if I even need this
+lean_object* cVec_boxer(cVec* v) {
+    return lean_alloc_external(g_cVec_external_class, v);
+}
+//good
+cVec* cVec_unboxer(lean_object* o) {
+    return (cVec*) lean_get_external_data(o);
+}
+
+//untested
+lean_object* cVec_struct_to_cVec_lean(cVec* c){
+    lean_object* out_arr = lean_mk_empty_array_with_capacity(lean_box_uint32(c->length));
+    for (size_t i = 0; i < c->length; i++){
+        out_arr = lean_array_push(out_arr, lean_box_float(c->data[i]));
+    }
+    return out_arr;
+}
+
+//untested
+cVec* cVec_lean_to_cVec_struct(lean_object* lean_arr) {
+    uint32_t arr_len = lean_array_size(lean_arr);   
+    cVec* v = cVec_alloc(sizeof(double) * arr_len);
+    v->length = arr_len;
+    for (size_t i = 0; i < arr_len; i++) {
+        v->data[i] = lean_unbox_float(lean_array_uget(lean_arr, i));
+    }
+    return v;
+}
+
+lean_object* cVec_new(lean_object* len_, double val) {
+    uint32_t len = lean_unbox_uint32(len_);
+    printf("len %u\n", len);
+
+    if (len == 0) {
+        return make_error("invalid length");
+    }
+
+    cVec* v = cVec_alloc(sizeof(double)*len);
+    if (!v) {
+        return make_error("ERROR_INSUF_MEM");
+    }
+    for (size_t i = 0; i < len; i++) {
+        v->data[i] = val;
+    }
+    lean_object* out_arr = lean_mk_empty_array_with_capacity(len_);
+    for (size_t i = 0; i < len; i++){
+        out_arr = lean_array_push(out_arr, lean_box_float(val));
+    }
+    return out_arr;
+}
+
+//good
+double cVec_get_val(lean_object* x_1, lean_object* x_2) {
+    lean_object* x_4; lean_object* x_5; 
+    x_4 = l_instInhabitedFloat;
+    x_5 = lean_array_get(x_4, x_1, x_2);
+    return lean_unbox_float(x_5);
+}
+//good
+double cVec_dot_prod(lean_object* lean_arr_v, lean_object* lean_arr_w){
+    double out = 0;
+    for (size_t i = 0; i < lean_array_size(lean_arr_v); i++){
+        out += lean_unbox_float(lean_array_uget(lean_arr_v, i)) * lean_unbox_float(lean_array_uget(lean_arr_w, i));
+    }
+    return out;
+}
