git/cruhland/lean4-axiomatic/Lean4Axiomatic/AbstractAlgebra/Core.lean
@@ -1,6 +1,6 @@
 import Lean4Axiomatic.Hand
 
-namespace Lean4Axiomatic.AA
+namespace Lean4Axiomatic
 
 /-!
 # Core definitions
@@ -9,21 +9,60 @@ These are used frequently by other abstract algebra definitions.
 -/
 
 /--
-Defines a convention for which side of a binary operator its first argument is
-sent to.
+Performs "alignment" of a heterogeneous binary operator.
 
-The given operator, of type `α → α → β`, is assumed to be left-handed; i.e.,
-its first argument is on the left when written infix. This function outputs a
-modified operator that puts the first argument on whatever side is specified by
-the `Hand` argument.
+By convention, binary operators are considered to be left-handed by default; in
+other words, their first arguments are always on the left when written infix.
+Right-hand alignment swaps the arguments, so that the first argument is given
+on the right with infix notation.
+
+This function outputs an operator that is equivalent to the one it receives as
+input, except that it will be aligned according to the `Hand` parameter. The
+input operator is assumed to be left-handed.
 
 This allows both the left- and right-handed versions of an algebraic property
 to share a single definition, avoiding repetitive code. See `AA.DistributiveOn`
 for an example.
+
+**Named parameters**
+- `α`: The `Sort` of the operator's first (default left) parameter.
+- `β`: The `Sort` of the operator's second (default right) parameter.
+- `γ`: The `Sort` of the operator's result.
+
+**Return type**: The return type contains what should be considered inputs to
+this function, but they are to the right of the colon so that they can be
+referenced in pattern matching. The first parameter is the `Hand` to use for
+alignment, and the second parameter is the operator to align. The rest of the
+return type denotes the output: the aligned version of the operator.
 -/
-def forHand {α : Sort u} {β : Sort v} : Hand → (α → α → β) → (α → α → β)
+abbrev Hand.hAlign
+    {α β : Sort u} {γ : Sort v}
+    : (hand : Hand) → (α → β → γ) → (hand.pick α β → hand.pick β α → γ)
 | Hand.L => id
 | Hand.R => flip
+
+/--
+Performs "alignment" of a homogeneous binary operator.
+
+This is a specialization of `Hand.hAlign` to operators whose left and right
+parameters have the same type (i.e., homogeneous operators). This is much more
+common than the heterogeneous case, so this definition exists for convenience.
+
+See `Hand.hAlign` for more details on the purpose of this function.
+
+**Named parameters**
+- `α`: The `Sort` of the operator's input parameters.
+- `β`: The `Sort` of the operator's result.
+
+**Return type**: The return type contains what should be considered inputs to
+this function, but they are to the right of the colon so that they can be
+referenced in pattern matching. The first parameter is the `Hand` to use for
+alignment, and the second parameter is the operator to align. The rest of the
+return type denotes the output: the aligned version of the operator.
+-/
+abbrev Hand.align {α : Sort u} {β : Sort v} : Hand → (α → α → β) → (α → α → β)
+| Hand.L => Hand.L.hAlign
+| Hand.R => Hand.R.hAlign
 
 /--
 The predicate that is always true.
@@ -33,6 +72,6 @@ this definition is to fill in constraint arguments of abstract algebra
 typeclasses when they're not needed. It's important that the name is as short
 as possible, to reduce clutter. See usages of `Substitutive₂` for examples.
 -/
-abbrev tc {α : Sort u} : α → Prop := λ _ => True
+abbrev AA.tc {α : Sort u} : α → Prop := λ _ => True
 
-end Lean4Axiomatic.AA
+end Lean4Axiomatic
