git/Augustindou/natural2lean-lean-project-template/LeanUtils/Parity.lean
@@ -2,10 +2,10 @@
 
 namespace Nat
   def even (a : Nat) : Prop := ∃ (n : Nat), a = 2 * n
-  def odd (a : Nat) : Prop := ¬ even a
+  def odd (a : Nat) : Prop := ∃ (n : Nat), a = 2 * n + 1
 end Nat
 
 namespace Int
   def even (a : Int) : Prop := ∃ (n : Int), a = 2 * n
-  def odd (a : Int) : Prop := ¬ even a
+  def odd (a : Int) : Prop := ∃ (n : Int), a = 2 * n + 1
 end Int
