git/Izzimach/qinglong/src/QingLong/EffIx.lean
@@ -1,0 +1,163 @@
+
+--
+-- Algebraic effects with indices, using the W-type
+--
+-- If you don't need the index consider Eff instead
+--
+
+
+import QingLong.PFunctor
+import QingLong.Wtype
+import QingLong.OpenUnion
+
+open pfunctor
+open Wtype
+open openunion
+
+namespace EffIx
+
+--
+-- ix should work like a Haskell Monoid. Here we used Inhabitied and HAdd for this functionality.
+--
+--inductive Eff (effs : List (Type → Type)) : Type → Type 1 where
+--    | Pure : α → Eff effs α
+--    | Impure : (γ : Type) → OU effs γ → (γ → Eff effs α) → Eff effs α
+
+inductive EffIxA (effs : List (Type → Type)) (α : Type) : Type 1 where
+    | Pure : α → EffIxA effs α 
+    | Impure : (x : Type) → OU effs x → EffIxA effs α -- the (x → W ..) part is in the second part of the pfunctor
+
+
+
+def EffIxB {effs : List (Type → Type)} {α : Type} : EffIxA effs α → Type
+    | .Pure a      => Fin 0 -- can't use False since we need a Type here, not a Prop
+    | .Impure x gx => x
+
+def EffIxPF (effs : List (Type → Type)) (α : Type) : pfunctor := pfunctor.mk (EffIxA effs α) (fun v => ULift <| EffIxB v)
+
+structure EffIxW {ix : Type} (effs : List (Type → Type)) (i : ix) (α : Type) : Type 1 where
+   val : W (EffIxPF effs α)
+
+
+-- lift into Eff.
+-- These universe shifts are annoying!
+def sendEff {α : Type} {g : Type → Type} {effs : List (Type → Type)} [HasEffect g effs] {ix : Type} (i : ix) (ga : g α) : EffIxW effs i α :=
+    EffIxW.mk <| ⟨EffIxA.Impure α (HasEffect.inject ga), fun a => W.mk ⟨EffIxA.Pure <| ULift.down a, Fin.elim0 ∘ ULift.down⟩⟩
+
+def pureEff {α : Type} {ix : Type} [Inhabited ix] (i : ix) (a : α) : EffIxW effs i α := EffIxW.mk ⟨EffIxA.Pure a, Fin.elim0 ∘ ULift.down⟩
+
+def bindEffW {effs : List (Type → Type)} {α β : Type} : W (EffIxPF effs α) → (α → W (EffIxPF effs β)) → W (EffIxPF effs β) := fun m1 m2 =>
+    match m1 with
+    | ⟨EffIxA.Pure a,     _⟩ => m2 a
+    | ⟨EffIxA.Impure x ou, bx⟩ => W.mk ⟨EffIxA.Impure x ou, fun x => (@bindEffW effs α β (bx x) m2)⟩
+
+def bindEff {α β ix : Type} [HAdd ix ix ix] {ix₁ ix₂ : ix}
+  : EffIxW g ix₁ α → (α → EffIxW g ix₂ β) → EffIxW g (ix₁ + ix₂) β := fun m1 m2 =>
+    -- we just strip off the FreerIxW wrapper and recurse
+    EffIxW.mk <| bindEffW m1.val (fun x => (m2 x).val)
+
+
+class IxMonad {ix : Type} (m : ix → Type → Type 1) where
+    pureIx : (i : ix) → α → m i α
+    bindIx [HAdd ix ix ix] : m i₁ α → (α → m i₂ β) → m (i₁ + i₂) β
+
+open IxMonad
+
+instance {ix : Type} [Inhabited ix] : @IxMonad ix (EffIxW effs) where
+    pureIx := fun i a => @pureEff effs _ ix _ i a
+    bindIx := bindEff
+
+
+
+--
+-- EffIxW as a Functor
+--
+
+def EffIxMap {ix : Type} {i : ix} (f : α → β) (w : EffIxW effs i α) : EffIxW effs i β :=
+    let Walg := fun d =>
+        match d with
+        | ⟨EffIxA.Pure a, z⟩         => W.mk ⟨EffIxA.Pure (f a), z⟩
+        | ⟨EffIxA.Impure x gx, next⟩ => W.mk ⟨EffIxA.Impure x gx, next⟩
+    EffIxW.mk <| Wtype.elim Walg w.val
+
+instance : Functor (EffIxW effs i) :=
+    { map := EffIxMap }
+
+
+
+-- Use the given collapser to convert an algebraic EffIxW monad into a static monad of type m. m is typically
+-- IO or StateIO s. For a pure result you could use Id for m.
+def interpretM {ix : Type} {i : ix} {α : Type} {m : Type → Type} [Monad m] (c : Collapser m effs) (tree : EffIxW effs i α) : m α :=
+    let Walg := fun zf =>
+        match zf with
+        | ⟨EffIxA.Pure a, _⟩ => ULift.up (pure a)
+        | ⟨EffIxA.Impure x gx, next⟩ => let a := do let z ← collapse c gx
+                                                    ULift.down (next <| ULift.up z)
+                                        ULift.up a
+    ULift.down <| Wtype.elim.{1} Walg tree.val
+
+
+
+
+
+
+inductive FReaderWriter (i : Type) (o : Type) : Type → Type where
+    | Get : FReaderWriter i o i
+    | Put : o → FReaderWriter i o Unit
+
+def collapseReaderWriter [StateOperator s "tag" Nat] (val : Nat) : ∀ x, FReaderWriter Nat Nat x → StateIO s x :=
+    fun x fr =>
+        match fr with
+        | FReaderWriter.Get => pure val
+        | FReaderWriter.Put v => fun s => pure ⟨(), StateOperator.putNamed "tag" v s⟩
+
+def getW [HasEffect (FReaderWriter Nat Nat) effs] : EffIxW effs 0 Nat := sendEff _ <| @FReaderWriter.Get Nat Nat
+def putW [HasEffect (FReaderWriter Nat Nat) effs] (v : Nat) : EffIxW effs 1 Unit := sendEff _ <| @FReaderWriter.Put Nat Nat v
+
+def evalIx {effs : List (Type → Type)} {ix : Type} {i : ix} {α : Type} : EffIxW effs i α → ix := fun _ => i
+
+-- if you have the collapser you can provide it to evalIx in order to help typeclass inference
+def evalIxC {effs : List (Type → Type)} {ix : Type} {i : ix} {α : Type} (c : Collapser m effs) (w : EffIxW effs i α) : ix := evalIx w
+
+structure StateTag where (tag : Nat)
+  deriving Repr
+
+instance : StateOperator StateTag "tag" Nat where
+  putNamed := fun n s => {s with tag := n}
+  getNamed := fun s => s.tag
+
+def rwCollapser {s : Type} [StateOperator s "tag" Nat] : Collapser (StateIO s) [FReaderWriter Nat Nat] :=
+    mkCollapse
+      @collapseReaderWriter s _ 3
+      o>
+
+def xCollapser := @rwCollapser StateTag _
+
+def xProg := bindIx (bindIx (getW) (fun x => putW 1)) (fun _ => @putW [FReaderWriter Nat Nat] _ 5)
+
+def x : StateIO StateTag Unit := (@interpretM _ _ _ Unit (StateIO StateTag) _ xCollapser <| xProg)
+
+def runX : StateTag → StateIO StateTag Unit → IO Nat :=
+  fun x s => do let ⟨a,s'⟩ ← s x
+                pure s'.tag
+
+#eval runX {tag := 2} x
+
+#eval evalIx <| xProg
+
+
+-- can't use normal do notation, so we make up a separate syntax for indexed monads
+
+syntax:60 term:60 " →→= " term:61 : term   -- >>= for indexed monads
+syntax:60 term:60 " →→ " term:61 : term   -- >>  for indexed monads
+
+macro_rules
+| `($l:term →→= $r:term) => `(bindIx $l $r)
+| `($l:term →→ $r:term) => `(bindIx $l (fun _ => $r))
+
+-- run the monad and output result
+#eval runX {tag := 2} <| interpretM xCollapser <| getW →→= putW →→ putW 3 →→ getW →→= putW
+
+-- should count # of putW's in the monad
+#eval evalIxC xCollapser <| getW →→= putW →→ getW →→= putW →→ putW 3
+
