git/Izzimach/qinglong/src/QingLong/FreerIxW.lean
@@ -1,0 +1,139 @@
+
+--
+-- Freer indexed monads built on the W-type
+--
+-- If you don't need the index consider FreerW instead
+--
+
+
+import QingLong.PFunctor
+import QingLong.Wtype
+
+open pfunctor
+open Wtype
+
+namespace FreerIxW
+
+--
+-- ix should work like a Haskell Monoid. Here we used Inhabitied and HAdd for this functionality.
+--
+-- data FFree g ix a where
+--   Pure :: {ix} → a → FFree g ix a
+--   Impure :: {ix} → g x → (x → FFree g a) → FFree g ix a
+
+inductive FreerIxA (g : Type → Type) (α : Type) : Type 1 where
+    | Pure : α → FreerIxA g α 
+    | Impure : (x : Type) → g x → FreerIxA g α -- the (x → W ..) part is in the second part of the pfunctor
+
+
+
+def FreerIxB {g : Type → Type} {α : Type} : FreerIxA g α → Type
+    | FreerIxA.Pure a => Fin 0 -- can't use False since we need a Type here, not a Prop
+    | FreerIxA.Impure x gx => x
+
+def FreerIxPF (g : Type → Type) (α : Type) : pfunctor := pfunctor.mk (FreerIxA g α) (fun v => ULift <| FreerIxB v)
+
+structure FreerIxW {ix : Type} (g : Type → Type) (i : ix) (α : Type) : Type 1 where
+   val : W (FreerIxPF g α)
+
+--
+-- FreerW as a Monad
+--
+
+-- lift into Free.
+-- These universe shifts are annoying!
+def liftFreer {α : Type} {g : Type → Type} {ix : Type} (i : ix) (ga : g α) : FreerIxW g i α :=
+    FreerIxW.mk <| ⟨FreerIxA.Impure α ga, fun a => W.mk ⟨FreerIxA.Pure <| ULift.down a, Fin.elim0 ∘ ULift.down⟩⟩
+
+def pureFreer {α : Type} {ix : Type} [Inhabited ix] (i : ix) (a : α) : FreerIxW g i α := FreerIxW.mk ⟨FreerIxA.Pure a, Fin.elim0 ∘ ULift.down⟩
+
+def bindFreerW {α β : Type} : W (FreerIxPF g α) → (α → W (FreerIxPF g β)) → W (FreerIxPF g β) := fun m1 m2 =>
+    match m1 with
+    | ⟨FreerIxA.Pure a,     _⟩ => m2 a
+    | ⟨FreerIxA.Impure x gx, bx⟩ =>W.mk ⟨FreerIxA.Impure x gx, fun x => (@bindFreerW g α β (bx x) m2)⟩
+
+def bindFreer {α β ix : Type} [HAdd ix ix ix] {ix₁ ix₂ : ix}
+  : FreerIxW g ix₁ α → (α → FreerIxW g ix₂ β) → FreerIxW g (ix₁ + ix₂) β := fun m1 m2 =>
+    -- we just strip off the FreerIxW wrapper and recurse
+    FreerIxW.mk <| bindFreerW m1.val (fun x => (m2 x).val)
+
+class IxMonad {ix : Type} (m : ix → Type → Type 1) where
+    pureIx : (i : ix) → α → m i α
+    bindIx [HAdd ix ix ix] : m i₁ α → (α → m i₂ β) → m (i₁ + i₂) β
+
+open IxMonad
+
+instance {ix : Type} [Inhabited ix] : @IxMonad ix (FreerIxW g) where
+    pureIx := fun i a => @pureFreer g _ ix _ i a
+    bindIx := bindFreer
+
+
+
+--
+-- FreerIxW as a Functor
+--
+
+def FreerIxMap {ix : Type} {i : ix} (f : α → β) (w : FreerIxW g i α) : FreerIxW g i β :=
+    let Walg := fun d =>
+        match d with
+        | ⟨FreerIxA.Pure a, z⟩         => W.mk ⟨FreerIxA.Pure (f a), z⟩
+        | ⟨FreerIxA.Impure x gx, next⟩ => W.mk ⟨FreerIxA.Impure x gx, next⟩
+    FreerIxW.mk <| Wtype.elim Walg w.val
+
+instance : Functor (FreerIxW f i) :=
+    { map := FreerIxMap }
+
+
+-- catamorphism threaded through the Freer structure
+def interpretW {ix : Type} {i : ix} {α : Type} {g : Type → Type} (alg : ∀ x, g x → x) (tree : FreerIxW g i α) : α :=
+    let Walg := fun zf =>
+        match zf with
+        | ⟨FreerIxA.Pure a, _⟩ => ULift.up a
+        | ⟨FreerIxA.Impure x gx, next⟩ => next <| ULift.up <| alg x gx
+    ULift.down <| Wtype.elim.{1} Walg tree.val
+
+def interpretM {ix : Type} {i : ix} {α : Type} {m g : Type → Type} [Monad m] (alg : ∀ x, g x → m x) (tree : FreerIxW g i α) : m α :=
+    let Walg := fun zf =>
+        match zf with
+        | ⟨FreerIxA.Pure a, _⟩ => ULift.up (pure a)
+        | ⟨FreerIxA.Impure x gx, next⟩ => let a := do let z ← alg x gx
+                                                      ULift.down (next <| ULift.up z)
+                                          ULift.up a
+    ULift.down <| Wtype.elim.{1} Walg tree.val
+
+
+inductive FReaderWriter (i : Type) (o : Type) : Type → Type where
+    | Get : FReaderWriter i o i
+    | Put : o → FReaderWriter i o Unit
+
+def runReaderWriter (val :Nat) (tree : FreerIxW (FReaderWriter Nat Nat) i α) : α :=
+  let alg := fun x fr =>
+      match fr with
+      | FReaderWriter.Get => val
+      | FReaderWriter.Put v => ()
+  interpretW alg tree
+
+def getW : FreerIxW (FReaderWriter Nat Nat) 0 Nat := liftFreer _ <| @FReaderWriter.Get Nat Nat
+def putW (v : Nat) : FreerIxW (FReaderWriter Nat Nat) 1 Unit := liftFreer _ <| @FReaderWriter.Put Nat Nat v
+
+def evalIx {g : Type → Type} {ix : Type} {i : ix} {α : Type} : FreerIxW g i α → ix := fun _ => i
+
+#eval runReaderWriter 4 <| bindIx (bindIx (getW) (fun x => putW x)) (fun _ => putW 3)
+#eval evalIx            <| bindIx (bindIx (getW) (fun x => putW x)) (fun _ => putW 3)
+
+
+-- can't use normal do notation, so we make up a separate syntax for indexed monads
+
+syntax:60 term:60 " ::→ " term:61 : term   -- >>= for indexed monads
+syntax:60 term:60 " **→ " term:61 : term   -- >>  for indexed monads
+
+macro_rules
+| `($l:term ::→ $r:term) => `(bindIx $l $r)
+| `($l:term **→ $r:term) => `(bindIx $l (fun _ => $r))
+
+-- run the monad and output result
+#eval runReaderWriter 6 <| getW ::→ putW **→ putW 3 **→ getW
+
+-- should count # of putW's in the monad
+#eval evalIx            <| getW ::→ putW **→ putW 3
+
