git/Izzimach/qinglong/src/QingLong/FreerW.lean
@@ -29,13 +29,23 @@ def untBump : (tBump x) → x
 
 def ZFreerBranch {g : Type → Type} {α : Type} : ZFreerPF g α → Type
     | ZFreerPF.ZPure a => Fin 0 -- can't use False since we need a Type here, not a Prop
-    | @ZFreerPF.ZImpure g α x gx => x
+    | ZFreerPF.ZImpure x gx => x
 
-def FreerPF (g : Type → Type) (α : Type) : pfunctor := pfunctor.mk (ZFreerPF g α) (fun x => tBump <| ZFreerBranch x)
+def FreerPF (g : Type → Type) (α : Type) : pfunctor := pfunctor.mk (ZFreerPF g α) (fun v => ULift <| ZFreerBranch v)
 
-def FreerW (g : Type → Type) (α : Type) := W (FreerPF g α)
+def FreerW (g : Type → Type) (α : Type) : Type 1 := W (FreerPF g α)
 
-def pureFreer {α : Type} (a : α) : FreerW g α := W.mk ⟨ZFreerPF.ZPure a, (fun ux => Fin.elim0 (untBump ux))⟩
+--
+-- FreerW as a Monad
+--
+
+-- lift into Free.
+-- These universe shifts are annoying!
+def liftFreer {α : Type} {g : Type → Type} (ga : g α) : FreerW g α :=
+    W.mk <| ⟨ZFreerPF.ZImpure α ga, fun a => W.mk ⟨ZFreerPF.ZPure <| ULift.down a, Fin.elim0 ∘ ULift.down⟩⟩
+
+def pureFreer {α : Type} (a : α) : FreerW g α := W.mk ⟨ZFreerPF.ZPure a, Fin.elim0 ∘ ULift.down⟩
+
 
 def bindFreer {α β : Type} (m1 : FreerW g α) (m2 : α → FreerW g β) : FreerW g β :=
     match m1 with
@@ -46,10 +56,45 @@ instance : Monad (FreerW g) where
     pure := pureFreer
     bind := bindFreer
 
+--
+-- FreerW as a Functor
+--
+
+def FreerMap (f : α → β) (w : FreerW g α) : FreerW g β :=
+    let Walg := fun d =>
+        match d with
+        | ⟨ZFreerPF.ZPure a, _⟩         => pureFreer <| f a
+        | ⟨ZFreerPF.ZImpure x gx, next⟩ => W.mk ⟨ZFreerPF.ZImpure x gx, next⟩ -- note, no FreerMap needed here...
+    Wtype.elim Walg w
+
+instance : Functor (FreerW f) :=
+    { map := FreerMap }
+
+
+-- catamorphism threaded through the Freer structure
+def interpretW {α : Type} {g : Type → Type} (alg : ∀ x, g x → x) (tree : FreerW g α) : α :=
+    let Walg := fun zf =>
+        match zf with
+        | ⟨ZFreerPF.ZPure a, _⟩ => ULift.up a
+        | ⟨ZFreerPF.ZImpure x gx, next⟩ => next <| ULift.up <| alg x gx
+    ULift.down <| Wtype.elim.{1} Walg tree
+
 
 inductive FReaderWriter (i : Type) (o : Type) : Type → Type where
     | Get : FReaderWriter i o i
     | Put : o → FReaderWriter i o Unit
+
+def runReaderWriter (val :Nat) (tree : FreerW (FReaderWriter Nat Nat) α) : α :=
+  let alg := fun x fr =>
+      match fr with
+      | FReaderWriter.Get => val
+      | FReaderWriter.Put v => ()
+  interpretW alg tree
+
+def getW := liftFreer <| @FReaderWriter.Get Nat Nat
+def putW (v : Nat) : FreerW (FReaderWriter Nat Nat) Unit := liftFreer <| @FReaderWriter.Put Nat Nat v
+
+#eval runReaderWriter 3 <| do let v ← getW; putW v; pure v
 
 def IT {x : Type} (i o α : Type) := FreerW (FReaderWriter i o) α
 
