git/Izzimach/qinglong/src/QingLong/OpenUnion.lean
@@ -26,13 +26,13 @@ elab "reflType" t:term : term => showType t
 
 
 inductive OU : List (Type → Type) → Type → Type 1 where
-  | Leaf : t x → OU (t :: effs) x
-  | Cons : OU effs x → OU (t :: effs) x
+    | Leaf : t x → OU (t :: effs) x
+    | Cons : OU effs x → OU (t :: effs) x
 
-def asStringOU (ou : OU r α) : String := 
-  match ou with
-  | OU.Leaf l => "Leaf"
-  | OU.Cons c => "Node/" ++ asStringOU c
+def asStringOU (ou : OU r α) : String :=
+    match ou with
+    | .Leaf l => "Leaf"
+    | .Cons c => "Node/" ++ asStringOU c
 
 instance [ToString x] : ToString (OU r x) where
     toString := asStringOU
@@ -53,3 +53,57 @@ instance [HasEffect r effs] : HasEffect (r : Type → Type) (x :: effs) where
                          | OU.Leaf l => Option.none
                          | OU.Cons c => HasEffect.project c
 
+
+
+
+
+inductive Collapser (m : Type → Type) : List (Type → Type) → Type 1 where
+    | End  : Collapser m []
+    | Cons : (∀x, t x → m x) → Collapser m effs → Collapser m (t :: effs)
+
+-- this is the annihilation of a sum type with a product type I always heard about
+def collapse {x : Type} {m : Type → Type} {effs : List (Type → Type)} (c : Collapser m (effs)) (ou : OU (effs) x) : m x :=
+    match c with
+    | .Cons alg n =>
+        match ou with
+        | .Leaf l => alg x l
+        | @OU.Cons effs' x _ ou' => collapse n ou'
+
+
+#check (Collapser.Cons (fun x v => pure (v : Id x)) (Collapser.Cons (fun x io => (io : IO x)) Collapser.End) : Collapser IO [Id, IO])
+
+
+def genCollapse (vals : List Syntax) : MetaM Syntax := do
+    match vals with
+    | List.cons h t => let pt ← genCollapse t
+                       `(Collapser.Cons $h $pt)
+    | List.nil      => `(Collapser.End)
+
+def elabCollapse (ts : Syntax.SepArray sep) : TermElabM Expr := do
+    let tsa : Array Syntax := ts
+    match tsa with
+    | Array.mk vals => let collapseStx ← (genCollapse vals)
+                       elabTerm collapseStx Option.none
+
+elab "mkCollapse " ts:term,+ " o> " : term => elabCollapse ts
+
+#check mkCollapse
+    (fun x v  => pure (v : Id x)) ,
+    (fun x io => (io : IO x))
+    o>
+
+def StateIO (sType : Type) (α : Type) : Type := sType → IO (α × sType)
+
+instance : Monad (StateIO s) where
+    pure := fun a s => pure ⟨a, s⟩
+    bind := fun m f s => do let ⟨a', s'⟩ ← m s
+                            f a' s'
+
+class StateOperator (stateContainer : Type) (name : String) (state : Type) where
+    putNamed : state → stateContainer → stateContainer
+    getNamed : stateContainer → state
+
+
+
+
+end openunion
