git/hargoniX/lean-ink-bug/Main.lean
@@ -1,0 +1,18 @@
+import LeanInk
+import Demo
+
+def main : IO Unit := do
+  let inputPath := System.FilePath.mk "Mathlib/Data/Option/Defs.lean"
+  let config := {
+    inputFilePath := inputPath
+    inputFileContents := (← IO.FS.readFile inputPath)
+    lakeFile := none
+    verbose := true
+    experimentalTypeInfo := true
+    experimentalDocString := true
+    experimentalSemanticType := true
+    prettifyOutput := true
+    : LeanInk.Configuration
+  }
+  let result ← LeanInk.Analysis.analyzeInput config
+  IO.println s!"Hello, {hello}!"
