git/zaxioms/LeanAlg/LeanAlg/Ffi.lean
@@ -1,0 +1,34 @@
+structure cVec where
+  data : Array Float
+
+instance : Inhabited (cVec) where
+  default : cVec := ⟨#[]⟩  
+
+namespace cVec
+
+#check cVec.mk
+
+#check cVec.data
+unsafe def externMk : Array Float -> cVec
+  := panic! "Can't actually do this"
+attribute [implementedBy externMk] cVec.mk
+
+unsafe def externData : cVec -> Array Float
+  := panic! "Can't actually do this"
+attribute [implementedBy externData] cVec.data
+
+@[extern "cVec_new"]
+def new (m : @&Nat) (x : @&Float) : cVec 
+  := ⟨mkArray m x⟩  
+
+def from_arr (a : @&Array Float) : cVec
+  := ⟨a⟩  
+
+@[extern "cVec_get_val"]
+def get (v : @&cVec) (i : @&Nat) : Float 
+  := v.data[i]
+
+@[extern "cVec_dot_prod"]
+def dot_product (v w : @&cVec) : Float
+  := Array.foldr (λ (x, y) z => z + x*y) 0 (Array.zip v.data w.data)
+
