git/zaxioms/LeanAlg/LeanAlg/Main.lean
@@ -1,0 +1,11 @@
+import Ffi
+
+#check 1.0 < 1.0 ∧ 1.0 > 1.0
+
+def main : IO Unit :=
+  do
+    let val := cVec.get (cVec.new 100 100) 99
+
+    let dot := cVec.dot_product (cVec.new 3 5) (cVec.new 3 3)
+    IO.eprintln s!"works"
+    IO.eprintln s!"{dot}"
